backend/CSEproof.v
@@ -1268,7 +1268,7 @@ Proof.
   exploit Mem.alloc_extends; eauto. apply Z.le_refl. apply Z.le_refl.
   intros (m'' & A & B).
   econstructor; split.
-  eapply exec_function_internal; simpl; eauto.
+  eapply exec_function_internal; simpl; eauto using Val.has_argtype_list_lessdef.
   simpl. econstructor; eauto.
   eapply analysis_correct_entry; eauto.
   apply init_regs_lessdef; auto.
