backend/CminorSel.v
@@ -434,6 +434,7 @@ Inductive step: state -> trace -> state -> Prop :=
         E0 (State f s' k' sp e m)
 
   | step_internal_function: forall f vargs k m m' sp e,
+      Val.has_argtype_list vargs f.(fn_sig).(sig_args) ->
       Mem.alloc m 0 f.(fn_stackspace) = (m', sp) ->
       set_locals f.(fn_vars) (set_params vargs f.(fn_params)) = e ->
       step (Callstate (Internal f) vargs k m)
