cfrontend/Cminorgenproof.v
@@ -2173,7 +2173,7 @@ Opaque PTree.set.
   exploit match_callstack_function_entry; eauto. simpl; eauto. simpl; auto.
   intros [f2 [MCS2 MINJ2]].
   left; econstructor; split.
-  apply plus_one. constructor; simpl; eauto.
+  apply plus_one. constructor; simpl; eauto using Val.has_argtype_list_inject.
   econstructor. eexact TRBODY. eauto. eexact MINJ2. eexact MCS2.
   inv MK; simpl in ISCC; contradiction || econstructor; eauto.
 
