cfrontend/Cshmgenproof.v
@@ -1384,6 +1384,14 @@ Proof.
   eapply make_cast_correct; eauto. eapply transl_expr_correct; eauto. auto.
 Qed.
 
+Lemma transl_arglist_typed:
+  forall al tyl vl,
+  Clight.eval_exprlist ge e le m al tyl vl ->
+  Val.has_argtype_list vl (List.map argtype_of_type tyl).
+Proof.
+  induction 1; intros; simpl; constructor; eauto using val_casted_has_argtype, cast_val_is_casted.
+Qed.
+
 Lemma typlist_of_arglist_eq:
   forall al tyl vl,
   Clight.eval_exprlist ge e le m al tyl vl ->
@@ -1492,7 +1500,8 @@ Inductive match_states: Clight.state -> Csharpminor.state -> Prop :=
           (TR: match_fundef cu fd tfd)
           (MK: match_cont ce tres 0%nat 0%nat k tk)
           (ISCC: Clight.is_call_cont k)
-          (TY: type_of_fundef fd = Tfunction targs tres cconv),
+          (TY: type_of_fundef fd = Tfunction targs tres cconv)
+          (CASTED: Val.has_argtype_list args (List.map argtype_of_type targs)),
       match_states (Clight.Callstate fd args k m)
                    (Callstate tfd args tk m)
   | match_returnstate:
@@ -1704,6 +1713,7 @@ Proof.
     econstructor; eauto.
     eapply match_Kcall with (ce := prog_comp_env cu') (cu := cu); eauto.
     exact I.
+    eapply transl_arglist_typed; eauto.
   + (* with normalization of return value *)
     subst optid.
     econstructor; split.
@@ -1715,6 +1725,7 @@ Proof.
     eapply match_Kcall_normalize  with (ce := prog_comp_env cu') (cu := cu); eauto.
     intros. eapply make_normalization_correct; eauto. constructor; eauto.
     exact I.
+    eapply transl_arglist_typed; eauto.
 
 - (* builtin *)
   monadInv TR. inv MTR.
@@ -1884,8 +1895,11 @@ Proof.
   exploit match_env_alloc_variables; eauto.
   apply match_env_empty.
   intros [te1 [C D]].
+  simpl in TY. unfold type_of_function in TY.
   econstructor; split.
   apply plus_one. eapply step_internal_function.
+  simpl. replace (map snd (Clight.fn_params f)) with targs. exact CASTED.
+  unfold type_of_params in TY; congruence.
   simpl. erewrite transl_vars_names by eauto. assumption.
   simpl. assumption.
   simpl. assumption.
@@ -1894,8 +1908,7 @@ Proof.
   simpl. econstructor; eauto.
   unfold transl_function. rewrite EQ; simpl. rewrite EQ1; simpl. auto.
   constructor.
-  replace (fn_return f) with tres. eassumption.
-  simpl in TY. unfold type_of_function in TY. congruence. 
+  replace (fn_return f) with tres. eassumption. congruence. 
 
 - (* external function *)
   inv TR.
@@ -1935,7 +1948,7 @@ Proof.
   { eapply transl_fundef_sig2; eauto. }
   econstructor; split.
   econstructor; eauto. apply (Genv.init_mem_match TRANSL). eauto.
-  econstructor; eauto. instantiate (1 := prog_comp_env cu). constructor; auto. exact I.
+  econstructor; eauto. instantiate (1 := prog_comp_env cu). constructor; auto. exact I. constructor.
 Qed.
 
 Lemma transl_final_states:
